Update RFJ

coq/rfj.v
@@ -4,50 +4,63 @@ Import ListNotations.
 Require Import MutualDistrust.fullabst.
 Require Import MutualDistrust.mutdist.
 
-(* Define RFJ *)
+(* Define RFJ interfaces *)
 
 Parameter rfj_class_declaration_table: Set.
 Parameter rfj_object_declaration_table: Set.
-Parameter rfj_class_definition_table: Set.
-Parameter rfj_object_definition_table: Set.
 
 Definition rfj_declaration_table: Set :=
   (rfj_class_declaration_table * rfj_object_declaration_table)%type.
-Definition rfj_definition_table: Set :=
-  (rfj_class_definition_table * rfj_object_definition_table)%type.
 
-Parameter has_interface:
-  rfj_declaration_table -> rfj_definition_table -> rfj_declaration_table -> Prop.
-
-Record rfj_component: Type :=
+Record rfj_interface: Set :=
   {
-    rfj_component_imports: rfj_declaration_table;
-    rfj_component_exports: rfj_declaration_table;
-    rfj_component_definitions: rfj_definition_table;
-    rfj_component_wf:
-      has_interface rfj_component_imports rfj_component_definitions rfj_component_exports
+    rfj_interface_imports: rfj_declaration_table;
+    rfj_interface_exports: rfj_declaration_table
   }.
 
-Parameter rfj_compatible2: rfj_component -> rfj_component -> Prop.
+Parameter rfj_compatible2: rfj_interface -> rfj_interface -> Prop.
 
-Inductive rfj_compatible: list rfj_component -> Prop :=
+Inductive rfj_compatible: list rfj_interface -> Prop :=
 | rfj_compatible_nil: rfj_compatible []
 | rfj_compatible_cons: forall C Cs,
                          rfj_compatible Cs ->
                          Forall (rfj_compatible2 C) Cs ->
                          rfj_compatible (C :: Cs).
 
-Definition rfj_program := list rfj_component.
+Parameter rfj_complete: list rfj_interface -> Prop.
 
-Parameter rfj_complete: rfj_program -> Prop.
+Instance rfji: interface_language rfj_interface :=
+  {
+    comp := fun Is => rfj_compatible Is /\ rfj_complete Is
+  }.
+
+(* Define RFJ *)
+
+Parameter rfj_class_definition_table: Set.
+Parameter rfj_object_definition_table: Set.
+
+Definition rfj_definition_table: Set :=
+  (rfj_class_definition_table * rfj_object_definition_table)%type.
+
+Parameter rfj_has_interface:
+  rfj_interface -> rfj_definition_table -> Prop.
+
+Record rfj_component: Type :=
+  {
+    rfj_component_interface: rfj_interface;
+    rfj_component_definitions: rfj_definition_table;
+    (* restrict to well-formed/well-typed components *)
+    rfj_component_wf:
+      rfj_has_interface rfj_component_interface rfj_component_definitions
+  }.
+
+Definition rfj_program := list rfj_component.
 
 Parameter rfj_beh_eq: rfj_program -> rfj_program -> Prop.
 
-(*
-Instance rfj : component_language rfj_component rfj_program :=
+Instance rfj : component_language rfji rfj_component rfj_program :=
   {
-    compatible := rfj_compatible;
-    complete := rfj_complete;
-    link := @id rfj_program;
+    has_interface := fun C I => rfj_component_interface C = I;
+    link := id;
     beh_eq := rfj_beh_eq
-  }.*)
+  }.
